LeanBF/Theory/Packing.lean
@@ -5,6 +5,7 @@ Authors: Bangyen Pham
 -/
 
 import LeanBF.Theory.Packing.Blocks
+import LeanBF.Theory.Packing.Divide
 import LeanBF.Theory.Packing.Support
 
 /-!
